\documentclass{article}
\usepackage{amsmath}

\begin{document}

\begin{align*}
    n \log n = \mathcal{O}(\log(n!)) \\
    &= \mathcal{O} \left(\frac{n}{2} \log n - \frac{n}{2} \log 2 \right) \\
    &= \mathcal{O} \left(\frac{n}{2} \log \frac{n}{2} \right) \\
    &= \mathcal{O} \left(\sum_{i = 0}^{\frac{n}{2}} \log \left(\frac{n}{2} + i\right) \right) \\
    &= \mathcal{O} \left(\sum_{i = \frac{n}{2}}^{n} \log i \right) \\
    &= \mathcal{O} \left(\sum_{i = 1}^{n} \log i - \sum_{i = 1}^{\frac{n}{2} - 1} \log i \right) \\
    &= \mathcal{O} \left(\log(n!) - \log \left(\left(\frac{n}{2} - 1\right)! \right) \right) \\
    &= \mathcal{O} \left(\log \left(\frac{n!}{(\frac{n}{2} - 1)!} \right) \right) \\
    &= \mathcal{O} \left(\log \prod_{i = \frac{n}{2}}^{n} i \right) \\
    &\text{(sloppily...)} \\
    = \mathcal{O}(\log(n!))
\end{align*}

\end{document}
